easy fixes

theories/Eq/Trace.v
@@ -1,7 +1,6 @@
 From Coq Require Import Basics.
 
-From Coinduction Require Import
-     coinduction rel tactics.
+From Coinduction Require Import all.
 
 From ITree Require Import Core.Subevent.
 From CTree Require Import
@@ -19,7 +18,7 @@ CoInductive trace {E} :=
 | Cons (l : @label E) (s : trace)
 | Nil.
 
-Program Definition htr {E C X} `{HasStuck : B0 -< C} :
+Program Definition htr {E C X} :
   mon (@trace E -> ctree E C X -> Prop) :=
   {| body R s t :=
     match s with
@@ -31,13 +30,13 @@ Next Obligation.
   destruct a. destruct H0 as (? & ? & ?). eauto. apply I.
 Defined.
 
-Definition has_trace {E C X} `{HasStuck : B0 -< C} := gfp (@htr E C X _).
+Definition has_trace {E C X} := gfp (@htr E C X).
 
-Definition tracincl {E C D X Y} `{B0 -< C} `{B0 -< D}
+Definition tracincl {E C D X Y}
   (t : ctree E C X) (t' : ctree E D Y) :=
   forall s, has_trace s t -> has_trace s t'.
 
-Definition traceq {E C D X Y} `{B0 -< C} `{B0 -< D}
+Definition traceq {E C D X Y}
   (t : ctree E C X) (t' : ctree E D Y) :=
   tracincl t t' /\ tracincl t' t.
 
@@ -45,12 +44,12 @@ Definition traceq {E C D X Y} `{B0 -< C} `{B0 -< D}
 Instances
 |*)
 
-#[global] Instance traceq_equ : forall {E C X} `{B0 -< C} s,
-  Proper (equ eq ==> impl) (@has_trace E C X _ s).
+#[global] Instance traceq_equ : forall {E C X} s,
+  Proper (equ eq ==> impl) (@has_trace E C X s).
 Proof.
   cbn. intros. step. destruct s; auto.
-  step in H1. cbn in H1. destruct H1 as (? & ? & ?).
-  rewrite H0 in H1. exists x0. auto.
+  step in H0. cbn in H0. destruct H0 as (? & ? & ?).
+  rewrite H in H0. exists x0. auto.
 Qed.
 
 (*|
@@ -73,18 +72,18 @@ Tactic Notation "__trace_play" "in" hyp(H) :=
 Trace inclusion is weaker than similarity,
 and trace equivalence is weaker than bisimilarity.
 |*)
-Lemma ssim_tracincl : forall {E C X} `{B0 -< C} (t t' : ctree E C X),
+Lemma ssim_tracincl : forall {E C X} (t t' : ctree E C X),
   ssim eq t t' -> tracincl t t'.
 Proof.
-  red. red. intros. revert t t' H0 s H1. coinduction R CH. intros.
+  red. red. intros. revert t t' H s H0. coinduction R CH. intros.
   simpl. destruct s; auto.
-  step in H1. cbn in H1. destruct H1 as (? & ? & ?).
-  step in H0. apply H0 in H1. destruct H1 as (? & ? & ? & ? & ?). subst.
-  exists x1. split. apply H1. eapply CH. apply H3. red. apply H2.
+  step in H0. cbn in H0. destruct H0 as (? & ? & ?).
+  step in H. apply H in H0. destruct H0 as (? & ? & ? & ? & ?). subst.
+  exists x1. split. apply H0. eapply CH. apply H2. red. apply H1.
 Qed.
 
-Lemma sbisim_traceq : forall {E C X} `{B0 -< C} (t t' : ctree E C X),
+Lemma sbisim_traceq : forall {E C X} (t t' : ctree E C X),
   sbisim eq t t' -> traceq t t'.
 Proof.
-  intros. split; apply ssim_tracincl; now apply sbisim_ssim.
+  intros. split; apply ssim_tracincl; now apply sbisim_ssim_subrelation.
 Qed.
